src/stage0/init/data/array/basic.cpp
@@ -18,14 +18,15 @@ obj* l_List_toArrayAux___rarg(obj*, obj*);
 obj* l___private_init_data_array_basic_1__iterateAux___main___rarg(obj*, obj*, obj*, obj*);
 obj* l_Array_toList___rarg___boxed(obj*);
 obj* l___private_init_data_array_basic_1__iterateAux___main___at_Array_map_u_2082___spec__1___boxed(obj*);
+obj* l_Array_empty___closed__1;
 namespace lean {
 obj* nat_sub(obj*, obj*);
 }
 obj* l___private_init_data_array_basic_2__revIterateAux___main___at_Array_toList___spec__1(obj*);
-obj* l_Array_Empty___rarg___boxed(obj*);
 obj* l_List_repr___rarg(obj*, obj*);
+obj* l_Array_update___boxed(obj*, obj*, obj*, obj*);
 obj* l_Array_revFoldl(obj*, obj*);
-obj* l_Array_write_x_27___boxed(obj*, obj*, obj*, obj*);
+obj* l_Array_isEmpty___boxed(obj*);
 obj* l___private_init_data_array_basic_2__revIterateAux___main___rarg(obj*, obj*, obj*, obj*, obj*);
 obj* l_Array_foreach___rarg(obj*, obj*);
 obj* l___private_init_data_array_basic_2__revIterateAux___main___at_Array_toList___spec__1___rarg(obj*, obj*, obj*, obj*, obj*);
@@ -34,54 +35,48 @@ obj* l___private_init_data_array_basic_1__iterateAux___main___at_Array_foreach__
 obj* l_Array_HasRepr(obj*);
 obj* l_Function_comp___rarg(obj*, obj*, obj*);
 obj* l_Array_iterate___boxed(obj*, obj*);
-obj* l_Array_uwrite___boxed(obj*, obj*, obj*, obj*, obj*);
 obj* l_Array_size___boxed(obj*, obj*);
 obj* l___private_init_data_array_basic_2__revIterateAux___main___boxed(obj*, obj*);
 obj* l___private_init_data_array_basic_1__iterateAux___main(obj*, obj*);
 obj* l___private_init_data_array_basic_1__iterateAux___main___at___private_init_data_array_basic_3__foreachAux___spec__1___rarg(obj*, obj*, obj*, obj*, obj*);
 obj* l___private_init_data_array_basic_2__revIterateAux___rarg(obj*, obj*, obj*, obj*, obj*);
-obj* l_Array_Empty___boxed(obj*);
 obj* l_List_toArrayAux___main___rarg(obj*, obj*);
-obj* l_Array_uread___boxed(obj*, obj*, obj*, obj*);
 obj* l_Array_foreach___boxed(obj*);
 obj* l___private_init_data_array_basic_2__revIterateAux___main(obj*, obj*);
-obj* l_Array_uwrite_x_27___boxed(obj*, obj*, obj*, obj*);
-obj* l_Array_read___boxed(obj*, obj*, obj*);
 obj* l_Array_pop___boxed(obj*, obj*);
 obj* l___private_init_data_array_basic_1__iterateAux___main___at___private_init_data_array_basic_3__foreachAux___spec__1(obj*);
 obj* l_Array_foreach(obj*);
 obj* l_List_toArrayAux___main___boxed(obj*);
 obj* l_List_toArrayAux(obj*);
-obj* l_Array_nil(obj*);
 obj* l_Array_toList___boxed(obj*);
 obj* l_Array_map___rarg(obj*, obj*);
 obj* l___private_init_data_array_basic_3__foreachAux(obj*);
+obj* l_Array_empty(obj*);
 obj* l___private_init_data_array_basic_1__iterateAux___main___at_Array_map_u_2082___spec__2___boxed(obj*);
+obj* l_Array_HasEmptyc(obj*);
 obj* l___private_init_data_array_basic_1__iterateAux___main___at_Array_map___spec__1___boxed(obj*);
 obj* l_Array_map_u_2082(obj*);
-obj* l_Array_Empty(obj*);
 obj* l_Array_toList___rarg(obj*);
+obj* l_Array_get___boxed(obj*, obj*, obj*, obj*);
 obj* l_Array_iterate(obj*, obj*);
 obj* l___private_init_data_array_basic_1__iterateAux___main___at_Array_map_u_2082___spec__2___rarg(obj*, obj*, obj*, obj*, obj*, obj*);
 obj* l___private_init_data_array_basic_2__revIterateAux___boxed(obj*, obj*);
 obj* l___private_init_data_array_basic_1__iterateAux___main___at_Array_map_u_2082___spec__1___rarg(obj*, obj*, obj*, obj*, obj*, obj*);
-obj* l_Array_nil___boxed(obj*);
 obj* l___private_init_data_array_basic_1__iterateAux___main___at_Array_foldl___spec__1(obj*, obj*);
 obj* l___private_init_data_array_basic_1__iterateAux___main___at_Array_map_u_2082___spec__2___rarg___boxed(obj*, obj*, obj*, obj*, obj*, obj*);
-obj* l_Array_mkNil___boxed(obj*, obj*);
 obj* l_List_toString___rarg(obj*, obj*);
 obj* l_Array_revIterate___boxed(obj*, obj*);
 obj* l_Array_revFoldl___rarg___boxed(obj*, obj*, obj*);
 namespace lean {
 uint8 nat_dec_lt(obj*, obj*);
 }
-obj* l_Array_write___boxed(obj*, obj*, obj*, obj*);
 obj* l___private_init_data_array_basic_1__iterateAux(obj*, obj*);
 obj* l___private_init_data_array_basic_1__iterateAux___main___at_Array_map___spec__1___rarg___boxed(obj*, obj*, obj*, obj*, obj*);
 obj* l_Array_foldl(obj*, obj*);
 obj* l___private_init_data_array_basic_2__revIterateAux___main___at_Array_revFoldl___spec__1___rarg___boxed(obj*, obj*, obj*, obj*, obj*, obj*);
 obj* l_Array_foldl___boxed(obj*, obj*);
 obj* l___private_init_data_array_basic_1__iterateAux___main___at_Array_foreach___spec__1___rarg(obj*, obj*, obj*, obj*, obj*);
+obj* l_Array_HasEmptyc___boxed(obj*);
 obj* l___private_init_data_array_basic_2__revIterateAux___main___at_Array_toList___spec__1___rarg___boxed(obj*, obj*, obj*, obj*, obj*);
 obj* l_Array_map_u_2082___boxed(obj*);
 namespace lean {
@@ -91,6 +86,7 @@ namespace lean {
 uint8 nat_dec_eq(obj*, obj*);
 }
 obj* l___private_init_data_array_basic_1__iterateAux___main___at_Array_map_u_2082___spec__1(obj*);
+uint8 l_Array_isEmpty___rarg(obj*);
 obj* l___private_init_data_array_basic_1__iterateAux___main___at_Array_map___spec__1(obj*);
 obj* l_Array_push___boxed(obj*, obj*, obj*);
 obj* l___private_init_data_array_basic_1__iterateAux___boxed(obj*, obj*);
@@ -105,20 +101,22 @@ obj* l_mkArray___boxed(obj*, obj*, obj*);
 obj* l_List_toArrayAux___boxed(obj*);
 obj* l_Array_revIterate___rarg(obj*, obj*, obj*);
 obj* l_Array_HasRepr___rarg___closed__1;
-obj* l_Array_uread_x_27___boxed(obj*, obj*, obj*, obj*);
 obj* l_Array_HasToString(obj*);
+obj* l_Array_updt___boxed(obj*, obj*, obj*, obj*, obj*);
 obj* l_List_toArray___boxed(obj*);
+obj* l_Array_isEmpty___rarg___boxed(obj*);
 obj* l___private_init_data_array_basic_1__iterateAux___main___boxed(obj*, obj*);
 obj* l_Array_iterate___rarg(obj*, obj*, obj*);
 obj* l___private_init_data_array_basic_1__iterateAux___main___at_Array_foreach___spec__1___boxed(obj*);
 obj* l_List_toArray___rarg(obj*);
+obj* l_Array_empty___boxed(obj*);
 obj* l_Array_HasToString___boxed(obj*);
 obj* l___private_init_data_array_basic_1__iterateAux___main___at___private_init_data_array_basic_3__foreachAux___spec__1___rarg___boxed(obj*, obj*, obj*, obj*, obj*);
-obj* l_Array_read_x_27___boxed(obj*, obj*, obj*, obj*);
 obj* l___private_init_data_array_basic_1__iterateAux___main___at___private_init_data_array_basic_3__foreachAux___spec__1___boxed(obj*);
 obj* l_Array_map_u_2082___rarg(obj*, obj*, obj*);
+obj* l_Array_isEmpty(obj*);
+obj* l_Array_index___boxed(obj*, obj*, obj*);
 obj* l_Array_revFoldl___boxed(obj*, obj*);
-obj* l_Array_nil___closed__1;
 obj* l_Array_HasRepr___boxed(obj*);
 obj* l_Array_HasRepr___rarg(obj*);
 namespace lean {
@@ -126,7 +124,6 @@ uint8 nat_dec_le(obj*, obj*);
 }
 obj* l_Array_revIterate___rarg___boxed(obj*, obj*, obj*);
 obj* l___private_init_data_array_basic_3__foreachAux___rarg(obj*, obj*);
-uint8 l_Array_Empty___rarg(obj*);
 obj* l___private_init_data_array_basic_1__iterateAux___main___at_Array_map___spec__1___rarg(obj*, obj*, obj*, obj*, obj*);
 obj* l_Array_HasToString___rarg(obj*);
 obj* l___private_init_data_array_basic_2__revIterateAux___rarg___boxed(obj*, obj*, obj*, obj*, obj*);
@@ -136,11 +133,14 @@ obj* l___private_init_data_array_basic_1__iterateAux___main___at_Array_foldl___s
 obj* l___private_init_data_array_basic_1__iterateAux___rarg(obj*, obj*, obj*, obj*);
 obj* l_Array_revIterate(obj*, obj*);
 obj* l_Array_toList(obj*);
+obj* l_Array_set___boxed(obj*, obj*, obj*, obj*);
 obj* l_Array_revFoldl___rarg(obj*, obj*, obj*);
+obj* l_Array_idx___boxed(obj*, obj*, obj*, obj*);
 obj* l_Array_foldl___rarg(obj*, obj*, obj*);
 obj* l_List_toArrayAux___main(obj*);
 obj* l___private_init_data_array_basic_2__revIterateAux___main___rarg___boxed(obj*, obj*, obj*, obj*, obj*);
 obj* l___private_init_data_array_basic_1__iterateAux___main___at_Array_foldl___spec__1___rarg___boxed(obj*, obj*, obj*, obj*, obj*);
+obj* l_Array_mkEmpty___boxed(obj*, obj*);
 obj* l___private_init_data_array_basic_1__iterateAux___main___at_Array_map_u_2082___spec__1___rarg___boxed(obj*, obj*, obj*, obj*, obj*, obj*);
 obj* l___private_init_data_array_basic_1__iterateAux___main___at_Array_foldl___spec__1___rarg(obj*, obj*, obj*, obj*, obj*);
 obj* l___private_init_data_array_basic_3__foreachAux___boxed(obj*);
@@ -161,41 +161,58 @@ x_3 = lean::mk_array(x_1, x_2);
 return x_3;
 }
 }
-obj* l_Array_mkNil___boxed(obj* x_0, obj* x_1) {
+obj* l_Array_mkEmpty___boxed(obj* x_0, obj* x_1) {
 _start:
 {
 obj* x_2; 
-x_2 = lean::mk_nil_array();
+x_2 = lean::mk_empty_array();
 return x_2;
 }
 }
-obj* _init_l_Array_nil___closed__1() {
+obj* _init_l_Array_empty___closed__1() {
 _start:
 {
 obj* x_0; obj* x_1; 
 x_0 = lean::box(0);
-x_1 = lean::mk_nil_array();
+x_1 = lean::mk_empty_array();
 return x_1;
 }
 }
-obj* l_Array_nil(obj* x_0) {
+obj* l_Array_empty(obj* x_0) {
 _start:
 {
 obj* x_1; 
-x_1 = l_Array_nil___closed__1;
+x_1 = l_Array_empty___closed__1;
 return x_1;
 }
 }
-obj* l_Array_nil___boxed(obj* x_0) {
+obj* l_Array_empty___boxed(obj* x_0) {
 _start:
 {
 obj* x_1; 
-x_1 = l_Array_nil(x_0);
+x_1 = l_Array_empty(x_0);
 lean::dec(x_0);
 return x_1;
 }
 }
-uint8 l_Array_Empty___rarg(obj* x_0) {
+obj* l_Array_HasEmptyc(obj* x_0) {
+_start:
+{
+obj* x_1; 
+x_1 = l_Array_empty___closed__1;
+return x_1;
+}
+}
+obj* l_Array_HasEmptyc___boxed(obj* x_0) {
+_start:
+{
+obj* x_1; 
+x_1 = l_Array_HasEmptyc(x_0);
+lean::dec(x_0);
+return x_1;
+}
+}
+uint8 l_Array_isEmpty___rarg(obj* x_0) {
 _start:
 {
 obj* x_1; obj* x_2; uint8 x_3; 
@@ -217,108 +234,90 @@ return x_6;
 }
 }
 }
-obj* l_Array_Empty(obj* x_0) {
+obj* l_Array_isEmpty(obj* x_0) {
 _start:
 {
 obj* x_1; 
-x_1 = lean::alloc_closure(reinterpret_cast<void*>(l_Array_Empty___rarg___boxed), 1, 0);
+x_1 = lean::alloc_closure(reinterpret_cast<void*>(l_Array_isEmpty___rarg___boxed), 1, 0);
 return x_1;
 }
 }
-obj* l_Array_Empty___rarg___boxed(obj* x_0) {
+obj* l_Array_isEmpty___rarg___boxed(obj* x_0) {
 _start:
 {
 uint8 x_1; obj* x_2; 
-x_1 = l_Array_Empty___rarg(x_0);
+x_1 = l_Array_isEmpty___rarg(x_0);
 x_2 = lean::box(x_1);
 lean::dec(x_0);
 return x_2;
 }
 }
-obj* l_Array_Empty___boxed(obj* x_0) {
+obj* l_Array_isEmpty___boxed(obj* x_0) {
 _start:
 {
 obj* x_1; 
-x_1 = l_Array_Empty(x_0);
+x_1 = l_Array_isEmpty(x_0);
 lean::dec(x_0);
 return x_1;
 }
 }
-obj* l_Array_read___boxed(obj* x_0, obj* x_1, obj* x_2) {
+obj* l_Array_index___boxed(obj* x_0, obj* x_1, obj* x_2) {
 _start:
 {
 obj* x_3; 
-x_3 = lean::array_read(x_1, x_2);
+x_3 = lean::array_index(x_1, x_2);
 lean::dec(x_1);
 lean::dec(x_2);
 return x_3;
 }
 }
-obj* l_Array_write___boxed(obj* x_0, obj* x_1, obj* x_2, obj* x_3) {
+obj* l_Array_idx___boxed(obj* x_0, obj* x_1, obj* x_2, obj* x_3) {
+_start:
+{
+usize x_4; obj* x_5; 
+x_4 = lean::unbox_size_t(x_2);
+x_5 = lean::array_idx(x_1, x_4);
+lean::dec(x_1);
+return x_5;
+}
+}
+obj* l_Array_get___boxed(obj* x_0, obj* x_1, obj* x_2, obj* x_3) {
 _start:
 {
 obj* x_4; 
-x_4 = lean::array_write(x_1, x_2, x_3);
-lean::dec(x_2);
-return x_4;
-}
-}
-obj* l_Array_read_x_27___boxed(obj* x_0, obj* x_1, obj* x_2, obj* x_3) {
-_start:
-{
-obj* x_4; 
-x_4 = lean::array_safe_read(x_1, x_2, x_3);
+x_4 = lean::array_get(x_1, x_2, x_3);
 lean::dec(x_2);
 lean::dec(x_3);
 return x_4;
 }
 }
-obj* l_Array_write_x_27___boxed(obj* x_0, obj* x_1, obj* x_2, obj* x_3) {
+obj* l_Array_update___boxed(obj* x_0, obj* x_1, obj* x_2, obj* x_3) {
 _start:
 {
 obj* x_4; 
-x_4 = lean::array_safe_write(x_1, x_2, x_3);
+x_4 = lean::array_update(x_1, x_2, x_3);
 lean::dec(x_2);
 return x_4;
 }
 }
-obj* l_Array_uread___boxed(obj* x_0, obj* x_1, obj* x_2, obj* x_3) {
-_start:
-{
-usize x_4; obj* x_5; 
-x_4 = lean::unbox_size_t(x_2);
-x_5 = lean::array_uread(x_1, x_4);
-lean::dec(x_1);
-return x_5;
-}
-}
-obj* l_Array_uwrite___boxed(obj* x_0, obj* x_1, obj* x_2, obj* x_3, obj* x_4) {
+obj* l_Array_updt___boxed(obj* x_0, obj* x_1, obj* x_2, obj* x_3, obj* x_4) {
 _start:
 {
 usize x_5; obj* x_6; 
 x_5 = lean::unbox_size_t(x_2);
-x_6 = lean::array_uwrite(x_1, x_5, x_3);
+x_6 = lean::array_updt(x_1, x_5, x_3);
 lean::dec(x_1);
 lean::dec(x_3);
 return x_6;
 }
 }
-obj* l_Array_uread_x_27___boxed(obj* x_0, obj* x_1, obj* x_2, obj* x_3) {
+obj* l_Array_set___boxed(obj* x_0, obj* x_1, obj* x_2, obj* x_3) {
 _start:
 {
-usize x_4; obj* x_5; 
-x_4 = lean::unbox_size_t(x_3);
-x_5 = lean::array_safe_uread(x_1, x_2, x_4);
-return x_5;
-}
-}
-obj* l_Array_uwrite_x_27___boxed(obj* x_0, obj* x_1, obj* x_2, obj* x_3) {
-_start:
-{
-usize x_4; obj* x_5; 
-x_4 = lean::unbox_size_t(x_2);
-x_5 = lean::array_safe_uwrite(x_1, x_4, x_3);
-return x_5;
+obj* x_4; 
+x_4 = lean::array_set(x_1, x_2, x_3);
+lean::dec(x_2);
+return x_4;
 }
 }
 obj* l_Array_push___boxed(obj* x_0, obj* x_1, obj* x_2) {
@@ -357,7 +356,7 @@ else
 obj* x_11; obj* x_12; obj* x_13; obj* x_15; 
 x_11 = lean::mk_nat_obj(1u);
 x_12 = lean::nat_add(x_2, x_11);
-x_13 = lean::array_read(x_0, x_2);
+x_13 = lean::array_index(x_0, x_2);
 lean::inc(x_1);
 x_15 = lean::apply_3(x_1, x_2, x_13, x_3);
 x_2 = x_12;
@@ -457,7 +456,7 @@ else
 obj* x_12; obj* x_13; obj* x_14; obj* x_17; 
 x_12 = lean::mk_nat_obj(1u);
 x_13 = lean::nat_add(x_3, x_12);
-x_14 = lean::array_read(x_2, x_3);
+x_14 = lean::array_index(x_2, x_3);
 lean::dec(x_3);
 lean::inc(x_1);
 x_17 = lean::apply_2(x_1, x_14, x_4);
@@ -535,7 +534,7 @@ obj* x_7; obj* x_8; obj* x_10; obj* x_13;
 x_7 = lean::mk_nat_obj(1u);
 x_8 = lean::nat_sub(x_2, x_7);
 lean::dec(x_2);
-x_10 = lean::array_read(x_0, x_8);
+x_10 = lean::array_index(x_0, x_8);
 lean::inc(x_8);
 lean::inc(x_1);
 x_13 = lean::apply_3(x_1, x_8, x_10, x_4);
@@ -664,7 +663,7 @@ obj* x_8; obj* x_9; obj* x_11; obj* x_13;
 x_8 = lean::mk_nat_obj(1u);
 x_9 = lean::nat_sub(x_3, x_8);
 lean::dec(x_3);
-x_11 = lean::array_read(x_2, x_9);
+x_11 = lean::array_index(x_2, x_9);
 lean::inc(x_1);
 x_13 = lean::apply_2(x_1, x_11, x_5);
 x_3 = x_9;
@@ -757,7 +756,7 @@ obj* x_7; obj* x_8; obj* x_10; obj* x_11;
 x_7 = lean::mk_nat_obj(1u);
 x_8 = lean::nat_sub(x_2, x_7);
 lean::dec(x_2);
-x_10 = lean::array_read(x_1, x_8);
+x_10 = lean::array_index(x_1, x_8);
 x_11 = lean::alloc_cnstr(1, 2, 0);
 lean::cnstr_set(x_11, 0, x_10);
 lean::cnstr_set(x_11, 1, x_4);
@@ -925,11 +924,11 @@ else
 obj* x_12; obj* x_13; obj* x_14; obj* x_17; obj* x_18; 
 x_12 = lean::mk_nat_obj(1u);
 x_13 = lean::nat_add(x_3, x_12);
-x_14 = lean::array_read(x_2, x_3);
+x_14 = lean::array_index(x_2, x_3);
 lean::inc(x_3);
 lean::inc(x_1);
 x_17 = lean::apply_2(x_1, x_3, x_14);
-x_18 = lean::array_write(x_4, x_3, x_17);
+x_18 = lean::array_update(x_4, x_3, x_17);
 lean::dec(x_3);
 x_3 = x_13;
 x_4 = x_18;
@@ -1012,11 +1011,11 @@ else
 obj* x_12; obj* x_13; obj* x_14; obj* x_17; obj* x_18; 
 x_12 = lean::mk_nat_obj(1u);
 x_13 = lean::nat_add(x_3, x_12);
-x_14 = lean::array_read(x_2, x_3);
+x_14 = lean::array_index(x_2, x_3);
 lean::inc(x_3);
 lean::inc(x_1);
 x_17 = lean::apply_2(x_1, x_3, x_14);
-x_18 = lean::array_write(x_4, x_3, x_17);
+x_18 = lean::array_update(x_4, x_3, x_17);
 lean::dec(x_3);
 x_3 = x_13;
 x_4 = x_18;
@@ -1099,10 +1098,10 @@ else
 obj* x_12; obj* x_13; obj* x_14; obj* x_16; obj* x_17; 
 x_12 = lean::mk_nat_obj(1u);
 x_13 = lean::nat_add(x_3, x_12);
-x_14 = lean::array_read(x_2, x_3);
+x_14 = lean::array_index(x_2, x_3);
 lean::inc(x_0);
 x_16 = lean::apply_1(x_0, x_14);
-x_17 = lean::array_write(x_4, x_3, x_16);
+x_17 = lean::array_update(x_4, x_3, x_16);
 lean::dec(x_3);
 x_3 = x_13;
 x_4 = x_17;
@@ -1185,11 +1184,11 @@ else
 obj* x_13; obj* x_14; obj* x_15; obj* x_16; obj* x_18; obj* x_19; 
 x_13 = lean::mk_nat_obj(1u);
 x_14 = lean::nat_add(x_4, x_13);
-x_15 = lean::array_read(x_3, x_4);
-x_16 = lean::array_read(x_1, x_4);
+x_15 = lean::array_index(x_3, x_4);
+x_16 = lean::array_index(x_1, x_4);
 lean::inc(x_0);
 x_18 = lean::apply_2(x_0, x_16, x_15);
-x_19 = lean::array_write(x_5, x_4, x_18);
+x_19 = lean::array_update(x_5, x_4, x_18);
 lean::dec(x_4);
 x_4 = x_14;
 x_5 = x_19;
@@ -1225,11 +1224,11 @@ else
 obj* x_13; obj* x_14; obj* x_15; obj* x_16; obj* x_18; obj* x_19; 
 x_13 = lean::mk_nat_obj(1u);
 x_14 = lean::nat_add(x_4, x_13);
-x_15 = lean::array_read(x_3, x_4);
-x_16 = lean::array_read(x_2, x_4);
+x_15 = lean::array_index(x_3, x_4);
+x_16 = lean::array_index(x_2, x_4);
 lean::inc(x_0);
 x_18 = lean::apply_2(x_0, x_16, x_15);
-x_19 = lean::array_write(x_5, x_4, x_18);
+x_19 = lean::array_update(x_5, x_4, x_18);
 lean::dec(x_4);
 x_4 = x_14;
 x_5 = x_19;
@@ -1401,7 +1400,7 @@ obj* l_List_toArray___rarg(obj* x_0) {
 _start:
 {
 obj* x_1; obj* x_2; 
-x_1 = l_Array_nil___closed__1;
+x_1 = l_Array_empty___closed__1;
 x_2 = l_List_toArrayAux___main___rarg(x_0, x_1);
 return x_2;
 }
@@ -1445,8 +1444,8 @@ if (io_result_is_error(w)) return w;
 w = initialize_init_function(w);
 if (io_result_is_error(w)) return w;
 w = initialize_init_data_tostring(w);
- l_Array_nil___closed__1 = _init_l_Array_nil___closed__1();
-lean::mark_persistent(l_Array_nil___closed__1);
+ l_Array_empty___closed__1 = _init_l_Array_empty___closed__1();
+lean::mark_persistent(l_Array_empty___closed__1);
  l_Array_HasRepr___rarg___closed__1 = _init_l_Array_HasRepr___rarg___closed__1();
 lean::mark_persistent(l_Array_HasRepr___rarg___closed__1);
 return w;
