src/stage0/init/data/dlist.cpp
@@ -14,44 +14,46 @@ typedef lean::uint32 uint32; typedef lean::uint64 uint64;
 #pragma GCC diagnostic ignored "-Wunused-label"
 #pragma GCC diagnostic ignored "-Wunused-but-set-variable"
 #endif
-obj* l_Dlist_cons___boxed(obj*);
-obj* l_Dlist_ofList___rarg(obj*);
-obj* l_Dlist_ofList(obj*);
-obj* l_Dlist_ofList___boxed(obj*);
+obj* l_DList_append(obj*);
+obj* l_DList_append___main(obj*);
+obj* l_DList_cons___main(obj*);
+obj* l_DList_push(obj*);
+obj* l_DList_toList___rarg(obj*);
+obj* l_DList_singleton___boxed(obj*);
 obj* l_Function_comp___rarg(obj*, obj*, obj*);
+obj* l_DList_HasEmptyc(obj*);
+obj* l_DList_toList___main___boxed(obj*);
+obj* l_DList_cons___rarg(obj*, obj*);
 obj* l_id___rarg___boxed(obj*);
-obj* l_Dlist_append___main(obj*);
-obj* l_Dlist_push___main___rarg(obj*, obj*, obj*);
-obj* l_Dlist_push___boxed(obj*);
-obj* l_Dlist_cons(obj*);
-obj* l_Dlist_Empty___boxed(obj*);
-obj* l_Dlist_HasAppend___boxed(obj*);
-obj* l_Dlist_cons___main___boxed(obj*);
-obj* l_Dlist_cons___main(obj*);
-obj* l_Dlist_toList___main___boxed(obj*);
-obj* l_Dlist_singleton(obj*);
-obj* l_Dlist_Empty(obj*);
-obj* l_Dlist_cons___rarg(obj*, obj*);
-obj* l_Dlist_append___main___boxed(obj*);
+obj* l_DList_singleton(obj*);
+obj* l_DList_toList(obj*);
+obj* l_DList_append___rarg(obj*, obj*);
+obj* l_DList_toList___main(obj*);
+obj* l_DList_append___main___boxed(obj*);
+obj* l_DList_cons___main___rarg(obj*, obj*, obj*);
+obj* l_DList_HasAppend(obj*);
+obj* l_DList_push___main___boxed(obj*);
+obj* l_DList_append___boxed(obj*);
 obj* l_List_append___rarg(obj*, obj*);
-obj* l_Dlist_push(obj*);
-obj* l_Dlist_singleton___rarg(obj*, obj*);
-obj* l_Dlist_toList___main___rarg(obj*);
-obj* l_Dlist_push___main(obj*);
-obj* l_Dlist_singleton___boxed(obj*);
-obj* l_Dlist_toList___main(obj*);
-obj* l_Dlist_toList(obj*);
-obj* l_Dlist_push___rarg(obj*, obj*);
-obj* l_Dlist_append___main___rarg(obj*, obj*);
-obj* l_Dlist_push___main___boxed(obj*);
-obj* l_Dlist_append___rarg(obj*, obj*);
-obj* l_Dlist_HasAppend(obj*);
-obj* l_Dlist_append(obj*);
-obj* l_Dlist_cons___main___rarg(obj*, obj*, obj*);
-obj* l_Dlist_toList___rarg(obj*);
-obj* l_Dlist_append___boxed(obj*);
-obj* l_Dlist_toList___boxed(obj*);
-obj* l_Dlist_ofList___rarg(obj* x_0) {
+obj* l_DList_push___boxed(obj*);
+obj* l_DList_cons(obj*);
+obj* l_DList_cons___main___boxed(obj*);
+obj* l_DList_toList___main___rarg(obj*);
+obj* l_DList_HasAppend___boxed(obj*);
+obj* l_DList_append___main___rarg(obj*, obj*);
+obj* l_DList_toList___boxed(obj*);
+obj* l_DList_empty(obj*);
+obj* l_DList_HasEmptyc___boxed(obj*);
+obj* l_DList_push___rarg(obj*, obj*);
+obj* l_DList_empty___boxed(obj*);
+obj* l_DList_cons___boxed(obj*);
+obj* l_DList_singleton___rarg(obj*, obj*);
+obj* l_DList_push___main___rarg(obj*, obj*, obj*);
+obj* l_DList_push___main(obj*);
+obj* l_DList_ofList(obj*);
+obj* l_DList_ofList___boxed(obj*);
+obj* l_DList_ofList___rarg(obj*);
+obj* l_DList_ofList___rarg(obj* x_0) {
 _start:
 {
 obj* x_1; 
@@ -60,24 +62,24 @@ lean::closure_set(x_1, 0, x_0);
 return x_1;
 }
 }
-obj* l_Dlist_ofList(obj* x_0) {
+obj* l_DList_ofList(obj* x_0) {
 _start:
 {
 obj* x_1; 
-x_1 = lean::alloc_closure(reinterpret_cast<void*>(l_Dlist_ofList___rarg), 1, 0);
+x_1 = lean::alloc_closure(reinterpret_cast<void*>(l_DList_ofList___rarg), 1, 0);
 return x_1;
 }
 }
-obj* l_Dlist_ofList___boxed(obj* x_0) {
+obj* l_DList_ofList___boxed(obj* x_0) {
 _start:
 {
 obj* x_1; 
-x_1 = l_Dlist_ofList(x_0);
+x_1 = l_DList_ofList(x_0);
 lean::dec(x_0);
 return x_1;
 }
 }
-obj* l_Dlist_Empty(obj* x_0) {
+obj* l_DList_empty(obj* x_0) {
 _start:
 {
 obj* x_1; 
@@ -85,16 +87,33 @@ x_1 = lean::alloc_closure(reinterpret_cast<void*>(l_id___rarg___boxed), 1, 0);
 return x_1;
 }
 }
-obj* l_Dlist_Empty___boxed(obj* x_0) {
+obj* l_DList_empty___boxed(obj* x_0) {
 _start:
 {
 obj* x_1; 
-x_1 = l_Dlist_Empty(x_0);
+x_1 = l_DList_empty(x_0);
 lean::dec(x_0);
 return x_1;
 }
 }
-obj* l_Dlist_toList___main___rarg(obj* x_0) {
+obj* l_DList_HasEmptyc(obj* x_0) {
+_start:
+{
+obj* x_1; 
+x_1 = lean::alloc_closure(reinterpret_cast<void*>(l_id___rarg___boxed), 1, 0);
+return x_1;
+}
+}
+obj* l_DList_HasEmptyc___boxed(obj* x_0) {
+_start:
+{
+obj* x_1; 
+x_1 = l_DList_HasEmptyc(x_0);
+lean::dec(x_0);
+return x_1;
+}
+}
+obj* l_DList_toList___main___rarg(obj* x_0) {
 _start:
 {
 obj* x_1; obj* x_2; 
@@ -103,49 +122,49 @@ x_2 = lean::apply_1(x_0, x_1);
 return x_2;
 }
 }
-obj* l_Dlist_toList___main(obj* x_0) {
+obj* l_DList_toList___main(obj* x_0) {
 _start:
 {
 obj* x_1; 
-x_1 = lean::alloc_closure(reinterpret_cast<void*>(l_Dlist_toList___main___rarg), 1, 0);
+x_1 = lean::alloc_closure(reinterpret_cast<void*>(l_DList_toList___main___rarg), 1, 0);
 return x_1;
 }
 }
-obj* l_Dlist_toList___main___boxed(obj* x_0) {
+obj* l_DList_toList___main___boxed(obj* x_0) {
 _start:
 {
 obj* x_1; 
-x_1 = l_Dlist_toList___main(x_0);
+x_1 = l_DList_toList___main(x_0);
 lean::dec(x_0);
 return x_1;
 }
 }
-obj* l_Dlist_toList___rarg(obj* x_0) {
+obj* l_DList_toList___rarg(obj* x_0) {
 _start:
 {
 obj* x_1; 
-x_1 = l_Dlist_toList___main___rarg(x_0);
+x_1 = l_DList_toList___main___rarg(x_0);
 return x_1;
 }
 }
-obj* l_Dlist_toList(obj* x_0) {
+obj* l_DList_toList(obj* x_0) {
 _start:
 {
 obj* x_1; 
-x_1 = lean::alloc_closure(reinterpret_cast<void*>(l_Dlist_toList___rarg), 1, 0);
+x_1 = lean::alloc_closure(reinterpret_cast<void*>(l_DList_toList___rarg), 1, 0);
 return x_1;
 }
 }
-obj* l_Dlist_toList___boxed(obj* x_0) {
+obj* l_DList_toList___boxed(obj* x_0) {
 _start:
 {
 obj* x_1; 
-x_1 = l_Dlist_toList(x_0);
+x_1 = l_DList_toList(x_0);
 lean::dec(x_0);
 return x_1;
 }
 }
-obj* l_Dlist_singleton___rarg(obj* x_0, obj* x_1) {
+obj* l_DList_singleton___rarg(obj* x_0, obj* x_1) {
 _start:
 {
 obj* x_2; 
@@ -155,24 +174,24 @@ lean::cnstr_set(x_2, 1, x_1);
 return x_2;
 }
 }
-obj* l_Dlist_singleton(obj* x_0) {
+obj* l_DList_singleton(obj* x_0) {
 _start:
 {
 obj* x_1; 
-x_1 = lean::alloc_closure(reinterpret_cast<void*>(l_Dlist_singleton___rarg), 2, 0);
+x_1 = lean::alloc_closure(reinterpret_cast<void*>(l_DList_singleton___rarg), 2, 0);
 return x_1;
 }
 }
-obj* l_Dlist_singleton___boxed(obj* x_0) {
+obj* l_DList_singleton___boxed(obj* x_0) {
 _start:
 {
 obj* x_1; 
-x_1 = l_Dlist_singleton(x_0);
+x_1 = l_DList_singleton(x_0);
 lean::dec(x_0);
 return x_1;
 }
 }
-obj* l_Dlist_cons___main___rarg(obj* x_0, obj* x_1, obj* x_2) {
+obj* l_DList_cons___main___rarg(obj* x_0, obj* x_1, obj* x_2) {
 _start:
 {
 obj* x_3; obj* x_4; 
@@ -183,78 +202,51 @@ lean::cnstr_set(x_4, 1, x_3);
 return x_4;
 }
 }
-obj* l_Dlist_cons___main(obj* x_0) {
+obj* l_DList_cons___main(obj* x_0) {
 _start:
 {
 obj* x_1; 
-x_1 = lean::alloc_closure(reinterpret_cast<void*>(l_Dlist_cons___main___rarg), 3, 0);
+x_1 = lean::alloc_closure(reinterpret_cast<void*>(l_DList_cons___main___rarg), 3, 0);
 return x_1;
 }
 }
-obj* l_Dlist_cons___main___boxed(obj* x_0) {
+obj* l_DList_cons___main___boxed(obj* x_0) {
 _start:
 {
 obj* x_1; 
-x_1 = l_Dlist_cons___main(x_0);
+x_1 = l_DList_cons___main(x_0);
 lean::dec(x_0);
 return x_1;
 }
 }
-obj* l_Dlist_cons___rarg(obj* x_0, obj* x_1) {
+obj* l_DList_cons___rarg(obj* x_0, obj* x_1) {
 _start:
 {
 obj* x_2; 
-x_2 = lean::alloc_closure(reinterpret_cast<void*>(l_Dlist_cons___main___rarg), 3, 2);
+x_2 = lean::alloc_closure(reinterpret_cast<void*>(l_DList_cons___main___rarg), 3, 2);
 lean::closure_set(x_2, 0, x_0);
 lean::closure_set(x_2, 1, x_1);
 return x_2;
 }
 }
-obj* l_Dlist_cons(obj* x_0) {
+obj* l_DList_cons(obj* x_0) {
 _start:
 {
 obj* x_1; 
-x_1 = lean::alloc_closure(reinterpret_cast<void*>(l_Dlist_cons___rarg), 2, 0);
+x_1 = lean::alloc_closure(reinterpret_cast<void*>(l_DList_cons___rarg), 2, 0);
 return x_1;
 }
 }
-obj* l_Dlist_cons___boxed(obj* x_0) {
+obj* l_DList_cons___boxed(obj* x_0) {
 _start:
 {
 obj* x_1; 
-x_1 = l_Dlist_cons(x_0);
+x_1 = l_DList_cons(x_0);
 lean::dec(x_0);
 return x_1;
 }
 }
-obj* l_Dlist_append___main___rarg(obj* x_0, obj* x_1) {
-_start:
-{
-obj* x_2; 
-x_2 = lean::alloc_closure(reinterpret_cast<void*>(l_Function_comp___rarg), 3, 2);
-lean::closure_set(x_2, 0, x_0);
-lean::closure_set(x_2, 1, x_1);
-return x_2;
-}
-}
-obj* l_Dlist_append___main(obj* x_0) {
-_start:
-{
-obj* x_1; 
-x_1 = lean::alloc_closure(reinterpret_cast<void*>(l_Dlist_append___main___rarg), 2, 0);
-return x_1;
-}
-}
-obj* l_Dlist_append___main___boxed(obj* x_0) {
-_start:
-{
-obj* x_1; 
-x_1 = l_Dlist_append___main(x_0);
-lean::dec(x_0);
-return x_1;
-}
-}
-obj* l_Dlist_append___rarg(obj* x_0, obj* x_1) {
+obj* l_DList_append___main___rarg(obj* x_0, obj* x_1) {
 _start:
 {
 obj* x_2; 
@@ -264,24 +256,51 @@ lean::closure_set(x_2, 1, x_1);
 return x_2;
 }
 }
-obj* l_Dlist_append(obj* x_0) {
+obj* l_DList_append___main(obj* x_0) {
 _start:
 {
 obj* x_1; 
-x_1 = lean::alloc_closure(reinterpret_cast<void*>(l_Dlist_append___rarg), 2, 0);
+x_1 = lean::alloc_closure(reinterpret_cast<void*>(l_DList_append___main___rarg), 2, 0);
 return x_1;
 }
 }
-obj* l_Dlist_append___boxed(obj* x_0) {
+obj* l_DList_append___main___boxed(obj* x_0) {
 _start:
 {
 obj* x_1; 
-x_1 = l_Dlist_append(x_0);
+x_1 = l_DList_append___main(x_0);
 lean::dec(x_0);
 return x_1;
 }
 }
-obj* l_Dlist_push___main___rarg(obj* x_0, obj* x_1, obj* x_2) {
+obj* l_DList_append___rarg(obj* x_0, obj* x_1) {
+_start:
+{
+obj* x_2; 
+x_2 = lean::alloc_closure(reinterpret_cast<void*>(l_Function_comp___rarg), 3, 2);
+lean::closure_set(x_2, 0, x_0);
+lean::closure_set(x_2, 1, x_1);
+return x_2;
+}
+}
+obj* l_DList_append(obj* x_0) {
+_start:
+{
+obj* x_1; 
+x_1 = lean::alloc_closure(reinterpret_cast<void*>(l_DList_append___rarg), 2, 0);
+return x_1;
+}
+}
+obj* l_DList_append___boxed(obj* x_0) {
+_start:
+{
+obj* x_1; 
+x_1 = l_DList_append(x_0);
+lean::dec(x_0);
+return x_1;
+}
+}
+obj* l_DList_push___main___rarg(obj* x_0, obj* x_1, obj* x_2) {
 _start:
 {
 obj* x_3; obj* x_4; 
@@ -292,63 +311,63 @@ x_4 = lean::apply_1(x_0, x_3);
 return x_4;
 }
 }
-obj* l_Dlist_push___main(obj* x_0) {
+obj* l_DList_push___main(obj* x_0) {
 _start:
 {
 obj* x_1; 
-x_1 = lean::alloc_closure(reinterpret_cast<void*>(l_Dlist_push___main___rarg), 3, 0);
+x_1 = lean::alloc_closure(reinterpret_cast<void*>(l_DList_push___main___rarg), 3, 0);
 return x_1;
 }
 }
-obj* l_Dlist_push___main___boxed(obj* x_0) {
+obj* l_DList_push___main___boxed(obj* x_0) {
 _start:
 {
 obj* x_1; 
-x_1 = l_Dlist_push___main(x_0);
+x_1 = l_DList_push___main(x_0);
 lean::dec(x_0);
 return x_1;
 }
 }
-obj* l_Dlist_push___rarg(obj* x_0, obj* x_1) {
+obj* l_DList_push___rarg(obj* x_0, obj* x_1) {
 _start:
 {
 obj* x_2; 
-x_2 = lean::alloc_closure(reinterpret_cast<void*>(l_Dlist_push___main___rarg), 3, 2);
+x_2 = lean::alloc_closure(reinterpret_cast<void*>(l_DList_push___main___rarg), 3, 2);
 lean::closure_set(x_2, 0, x_0);
 lean::closure_set(x_2, 1, x_1);
 return x_2;
 }
 }
-obj* l_Dlist_push(obj* x_0) {
+obj* l_DList_push(obj* x_0) {
 _start:
 {
 obj* x_1; 
-x_1 = lean::alloc_closure(reinterpret_cast<void*>(l_Dlist_push___rarg), 2, 0);
+x_1 = lean::alloc_closure(reinterpret_cast<void*>(l_DList_push___rarg), 2, 0);
 return x_1;
 }
 }
-obj* l_Dlist_push___boxed(obj* x_0) {
+obj* l_DList_push___boxed(obj* x_0) {
 _start:
 {
 obj* x_1; 
-x_1 = l_Dlist_push(x_0);
+x_1 = l_DList_push(x_0);
 lean::dec(x_0);
 return x_1;
 }
 }
-obj* l_Dlist_HasAppend(obj* x_0) {
+obj* l_DList_HasAppend(obj* x_0) {
 _start:
 {
 obj* x_1; 
-x_1 = lean::alloc_closure(reinterpret_cast<void*>(l_Dlist_append___rarg), 2, 0);
+x_1 = lean::alloc_closure(reinterpret_cast<void*>(l_DList_append___rarg), 2, 0);
 return x_1;
 }
 }
-obj* l_Dlist_HasAppend___boxed(obj* x_0) {
+obj* l_DList_HasAppend___boxed(obj* x_0) {
 _start:
 {
 obj* x_1; 
-x_1 = l_Dlist_HasAppend(x_0);
+x_1 = l_DList_HasAppend(x_0);
 lean::dec(x_0);
 return x_1;
 }
