src/stage0/init/data/hashmap/basic.cpp
@@ -14,27 +14,25 @@ typedef lean::uint32 uint32; typedef lean::uint64 uint64;
 #pragma GCC diagnostic ignored "-Wunused-label"
 #pragma GCC diagnostic ignored "-Wunused-but-set-variable"
 #endif
-obj* l_DHashmap_Empty___boxed(obj*, obj*, obj*, obj*);
-obj* l_DHashmap_Empty(obj*, obj*, obj*, obj*);
 obj* l_HashmapImp_findAux___rarg(obj*, obj*, obj*);
 obj* l_HashmapImp_fold(obj*, obj*, obj*);
 obj* l_HashmapImp_replaceAux___main___boxed(obj*, obj*);
 obj* l_HashmapImp_replaceAux___main___rarg(obj*, obj*, obj*, obj*);
 obj* l_Hashmap_fold___rarg(obj*, obj*, obj*);
+uint8 l_Hashmap_empty___rarg(obj*);
+obj* l_DHashmap_empty___boxed(obj*, obj*, obj*, obj*);
 obj* l_DHashmap_find(obj*, obj*);
-obj* l_Hashmap_Empty(obj*, obj*, obj*, obj*);
 obj* l_DHashmap_contains___rarg___boxed(obj*, obj*, obj*, obj*);
 namespace lean {
 obj* nat_sub(obj*, obj*);
 }
 obj* l_Hashmap_erase___rarg(obj*, obj*, obj*, obj*);
 obj* l_DHashmap_insert(obj*, obj*);
+obj* l_Hashmap_empty___boxed(obj*, obj*, obj*, obj*);
 obj* l_HashmapImp_insert(obj*, obj*);
 uint8 l_Option_isSome___main___rarg(obj*);
-obj* l_bucketArray_uwrite(obj*, obj*);
 obj* l_HashmapImp_foldBuckets___boxed(obj*, obj*, obj*);
 obj* l_HashmapImp_reinsertAux(obj*, obj*);
-obj* l_bucketArray_uwrite___boxed(obj*, obj*);
 obj* l___private_init_data_array_basic_1__iterateAux___main___at_HashmapImp_foldBuckets___spec__2___rarg___boxed(obj*, obj*, obj*, obj*, obj*);
 uint8 l_HashmapImp_containsAux___rarg(obj*, obj*, obj*);
 obj* l_Hashmap_find___rarg(obj*, obj*, obj*, obj*);
@@ -49,21 +47,22 @@ obj* l_mkHashmapImp(obj*, obj*);
 obj* l_Hashmap_erase___boxed(obj*, obj*);
 obj* l_HashmapImp_erase(obj*, obj*);
 obj* l_DHashmap_contains(obj*, obj*);
-obj* l_bucketArray_uwrite___rarg(obj*, usize, obj*, obj*);
 obj* l_DHashmap_insert___rarg(obj*, obj*, obj*, obj*, obj*);
 obj* l_HashmapImp_find(obj*, obj*);
 obj* l_HashmapImp_mkIdx___boxed(obj*, obj*, obj*);
+obj* l_bucketArray_updt___rarg(obj*, usize, obj*, obj*);
 obj* l_HashmapImp_replaceAux___boxed(obj*, obj*);
 obj* l_List_foldl___main___at_HashmapImp_foldBuckets___spec__1___boxed(obj*, obj*, obj*);
 obj* l_HashmapImp_findAux___main___rarg(obj*, obj*, obj*);
 obj* l___private_init_data_array_basic_1__iterateAux___main___at_HashmapImp_foldBuckets___spec__2___boxed(obj*, obj*, obj*);
 obj* l_HashmapImp_fold___rarg(obj*, obj*, obj*);
 obj* l_HashmapImp_erase___boxed(obj*, obj*);
-uint8 l_Hashmap_Empty___rarg(obj*);
 obj* l_HashmapImp_containsAux___boxed(obj*, obj*);
 obj* l_DHashmap_fold(obj*, obj*, obj*, obj*, obj*);
 obj* l_Hashmap_fold___boxed(obj*, obj*, obj*, obj*, obj*);
+obj* l_bucketArray_updt(obj*, obj*);
 obj* l_mkHashmap___boxed(obj*, obj*, obj*, obj*);
+obj* l_DHashmap_empty___rarg___boxed(obj*);
 obj* l_DHashmap_erase(obj*, obj*);
 obj* l_DHashmap_contains___boxed(obj*, obj*);
 obj* l_Hashmap_insert___boxed(obj*, obj*);
@@ -75,7 +74,6 @@ obj* l_HashmapImp_insert___boxed(obj*, obj*);
 obj* l_HashmapImp_replaceAux___rarg(obj*, obj*, obj*, obj*);
 obj* l_HashmapImp_findAux(obj*, obj*);
 obj* l_HashmapImp_insert___rarg(obj*, obj*, obj*, obj*, obj*);
-obj* l_Hashmap_Empty___rarg___boxed(obj*);
 obj* l_DHashmap_size(obj*, obj*, obj*, obj*);
 obj* l_HashmapImp_erase___rarg(obj*, obj*, obj*, obj*);
 obj* l_List_foldl___main___at_HashmapImp_foldBuckets___spec__1(obj*, obj*, obj*);
@@ -92,25 +90,26 @@ obj* nat_add(obj*, obj*);
 }
 obj* l_DHashmap_insert___boxed(obj*, obj*);
 obj* l_Hashmap_find(obj*, obj*);
+uint8 l_DHashmap_empty___rarg(obj*);
 namespace lean {
 uint8 nat_dec_eq(obj*, obj*);
 }
 obj* l_DHashmap_size___rarg(obj*);
 obj* l_HashmapImp_foldBuckets___rarg(obj*, obj*, obj*);
+obj* l_Hashmap_empty(obj*, obj*, obj*, obj*);
 obj* l_HashmapImp_containsAux___rarg___boxed(obj*, obj*, obj*);
+obj* l_Hashmap_empty___rarg___boxed(obj*);
 obj* l_Hashmap_fold(obj*, obj*, obj*, obj*, obj*);
 obj* l_Hashmap_contains(obj*, obj*);
 obj* l_Hashmap_size___rarg___boxed(obj*);
 obj* l_HashmapImp_findAux___boxed(obj*, obj*);
-obj* l_DHashmap_Empty___rarg___boxed(obj*);
+obj* l_bucketArray_updt___rarg___boxed(obj*, obj*, obj*, obj*);
 obj* l_mkDHashmap(obj*, obj*, obj*, obj*);
 obj* l_mkDHashmap___rarg(obj*);
 obj* l_Hashmap_insert(obj*, obj*);
 obj* l_HashmapImp_eraseAux___rarg(obj*, obj*, obj*);
-uint8 l_DHashmap_Empty___rarg(obj*);
 obj* l_Hashmap_find___boxed(obj*, obj*);
 obj* l_Hashmap_contains___rarg___boxed(obj*, obj*, obj*, obj*);
-obj* l_bucketArray_uwrite___rarg___boxed(obj*, obj*, obj*, obj*);
 obj* l_HashmapImp_eraseAux___main(obj*, obj*);
 obj* l_DHashmap_size___rarg___boxed(obj*);
 namespace lean {
@@ -129,12 +128,13 @@ uint8 nat_dec_le(obj*, obj*);
 }
 obj* l_DHashmap_find___rarg(obj*, obj*, obj*, obj*);
 obj* l_mkHashmapImp___rarg___closed__1;
-obj* l_Hashmap_Empty___boxed(obj*, obj*, obj*, obj*);
 obj* l_List_foldl___main___at_HashmapImp_foldBuckets___spec__1___rarg(obj*, obj*, obj*);
 obj* l_Hashmap_insert___rarg(obj*, obj*, obj*, obj*, obj*);
 obj* l_HashmapImp_foldBuckets(obj*, obj*, obj*);
+obj* l_DHashmap_empty(obj*, obj*, obj*, obj*);
 obj* l_DHashmap_fold___boxed(obj*, obj*, obj*, obj*, obj*);
 obj* l_DHashmap_fold___rarg(obj*, obj*, obj*);
+obj* l_bucketArray_updt___boxed(obj*, obj*);
 obj* l___private_init_data_array_basic_1__iterateAux___main___at_HashmapImp_foldBuckets___spec__2(obj*, obj*, obj*);
 obj* l_DHashmap_erase___rarg(obj*, obj*, obj*, obj*);
 obj* l_HashmapImp_fold___boxed(obj*, obj*, obj*);
@@ -147,39 +147,39 @@ obj* nat_mul(obj*, obj*);
 obj* l_HashmapImp_replaceAux(obj*, obj*);
 obj* l_HashmapImp_eraseAux___main___rarg(obj*, obj*, obj*);
 obj* l_HashmapImp_findAux___main___boxed(obj*, obj*);
-obj* l_bucketArray_uwrite___rarg(obj* x_0, usize x_1, obj* x_2, obj* x_3) {
+obj* l_bucketArray_updt___rarg(obj* x_0, usize x_1, obj* x_2, obj* x_3) {
 _start:
 {
 obj* x_4; 
-x_4 = lean::array_uwrite(x_0, x_1, x_2);
+x_4 = lean::array_updt(x_0, x_1, x_2);
 return x_4;
 }
 }
-obj* l_bucketArray_uwrite(obj* x_0, obj* x_1) {
+obj* l_bucketArray_updt(obj* x_0, obj* x_1) {
 _start:
 {
 obj* x_2; 
-x_2 = lean::alloc_closure(reinterpret_cast<void*>(l_bucketArray_uwrite___rarg___boxed), 4, 0);
+x_2 = lean::alloc_closure(reinterpret_cast<void*>(l_bucketArray_updt___rarg___boxed), 4, 0);
 return x_2;
 }
 }
-obj* l_bucketArray_uwrite___rarg___boxed(obj* x_0, obj* x_1, obj* x_2, obj* x_3) {
+obj* l_bucketArray_updt___rarg___boxed(obj* x_0, obj* x_1, obj* x_2, obj* x_3) {
 _start:
 {
 usize x_4; obj* x_5; 
 x_4 = lean::unbox_size_t(x_1);
-x_5 = l_bucketArray_uwrite___rarg(x_0, x_4, x_2, x_3);
+x_5 = l_bucketArray_updt___rarg(x_0, x_4, x_2, x_3);
 lean::dec(x_0);
 lean::dec(x_2);
 lean::dec(x_3);
 return x_5;
 }
 }
-obj* l_bucketArray_uwrite___boxed(obj* x_0, obj* x_1) {
+obj* l_bucketArray_updt___boxed(obj* x_0, obj* x_1) {
 _start:
 {
 obj* x_2; 
-x_2 = l_bucketArray_uwrite(x_0, x_1);
+x_2 = l_bucketArray_updt(x_0, x_1);
 lean::dec(x_0);
 lean::dec(x_1);
 return x_2;
@@ -276,11 +276,11 @@ lean::dec(x_5);
 x_11 = lean::alloc_cnstr(0, 2, 0);
 lean::cnstr_set(x_11, 0, x_2);
 lean::cnstr_set(x_11, 1, x_3);
-x_12 = lean::array_uread(x_1, x_9);
+x_12 = lean::array_idx(x_1, x_9);
 x_13 = lean::alloc_cnstr(1, 2, 0);
 lean::cnstr_set(x_13, 0, x_11);
 lean::cnstr_set(x_13, 1, x_12);
-x_14 = lean::array_uwrite(x_1, x_9, x_13);
+x_14 = lean::array_updt(x_1, x_9, x_13);
 lean::dec(x_13);
 lean::dec(x_1);
 return x_14;
@@ -361,7 +361,7 @@ else
 obj* x_12; obj* x_13; obj* x_14; obj* x_17; 
 x_12 = lean::mk_nat_obj(1u);
 x_13 = lean::nat_add(x_3, x_12);
-x_14 = lean::array_read(x_2, x_3);
+x_14 = lean::array_index(x_2, x_3);
 lean::dec(x_3);
 lean::inc(x_1);
 x_17 = l_List_foldl___main___at_HashmapImp_foldBuckets___spec__1___rarg(x_1, x_4, x_14);
@@ -582,7 +582,7 @@ x_10 = lean::apply_1(x_1, x_3);
 x_11 = lean::unbox_size_t(x_10);
 x_12 = lean::usize_modn(x_11, x_8);
 lean::dec(x_8);
-x_14 = lean::array_uread(x_4, x_12);
+x_14 = lean::array_idx(x_4, x_12);
 lean::dec(x_4);
 x_16 = l_HashmapImp_findAux___main___rarg(x_0, x_3, x_14);
 return x_16;
@@ -879,7 +879,7 @@ lean::inc(x_1);
 x_14 = lean::apply_1(x_1, x_3);
 x_15 = lean::unbox_size_t(x_14);
 x_16 = lean::usize_modn(x_15, x_11);
-x_17 = lean::array_uread(x_7, x_16);
+x_17 = lean::array_idx(x_7, x_16);
 lean::inc(x_17);
 lean::inc(x_3);
 lean::inc(x_0);
@@ -897,7 +897,7 @@ lean::cnstr_set(x_26, 1, x_4);
 x_27 = lean::alloc_cnstr(1, 2, 0);
 lean::cnstr_set(x_27, 0, x_26);
 lean::cnstr_set(x_27, 1, x_17);
-x_28 = lean::array_uwrite(x_7, x_16, x_27);
+x_28 = lean::array_updt(x_7, x_16, x_27);
 lean::dec(x_27);
 lean::dec(x_7);
 x_31 = lean::nat_dec_le(x_24, x_11);
@@ -945,7 +945,7 @@ obj* x_48; obj* x_49; obj* x_52;
 lean::dec(x_11);
 lean::dec(x_1);
 x_48 = l_HashmapImp_replaceAux___main___rarg(x_0, x_3, x_4, x_17);
-x_49 = lean::array_uwrite(x_7, x_16, x_48);
+x_49 = lean::array_updt(x_7, x_16, x_48);
 lean::dec(x_48);
 lean::dec(x_7);
 if (lean::is_scalar(x_9)) {
@@ -992,7 +992,7 @@ x_11 = lean::apply_1(x_1, x_3);
 x_12 = lean::unbox_size_t(x_11);
 x_13 = lean::usize_modn(x_12, x_9);
 lean::dec(x_9);
-x_15 = lean::array_uread(x_6, x_13);
+x_15 = lean::array_idx(x_6, x_13);
 lean::inc(x_15);
 lean::inc(x_3);
 lean::inc(x_0);
@@ -1021,7 +1021,7 @@ x_26 = lean::mk_nat_obj(1u);
 x_27 = lean::nat_sub(x_4, x_26);
 lean::dec(x_4);
 x_29 = l_HashmapImp_eraseAux___main___rarg(x_0, x_3, x_15);
-x_30 = lean::array_uwrite(x_6, x_13, x_29);
+x_30 = lean::array_updt(x_6, x_13, x_29);
 lean::dec(x_29);
 lean::dec(x_6);
 if (lean::is_scalar(x_25)) {
@@ -1263,7 +1263,7 @@ lean::dec(x_3);
 return x_4;
 }
 }
-uint8 l_DHashmap_Empty___rarg(obj* x_0) {
+uint8 l_DHashmap_empty___rarg(obj* x_0) {
 _start:
 {
 obj* x_1; obj* x_2; uint8 x_3; 
@@ -1285,29 +1285,29 @@ return x_6;
 }
 }
 }
-obj* l_DHashmap_Empty(obj* x_0, obj* x_1, obj* x_2, obj* x_3) {
+obj* l_DHashmap_empty(obj* x_0, obj* x_1, obj* x_2, obj* x_3) {
 _start:
 {
 obj* x_4; 
-x_4 = lean::alloc_closure(reinterpret_cast<void*>(l_DHashmap_Empty___rarg___boxed), 1, 0);
+x_4 = lean::alloc_closure(reinterpret_cast<void*>(l_DHashmap_empty___rarg___boxed), 1, 0);
 return x_4;
 }
 }
-obj* l_DHashmap_Empty___rarg___boxed(obj* x_0) {
+obj* l_DHashmap_empty___rarg___boxed(obj* x_0) {
 _start:
 {
 uint8 x_1; obj* x_2; 
-x_1 = l_DHashmap_Empty___rarg(x_0);
+x_1 = l_DHashmap_empty___rarg(x_0);
 x_2 = lean::box(x_1);
 lean::dec(x_0);
 return x_2;
 }
 }
-obj* l_DHashmap_Empty___boxed(obj* x_0, obj* x_1, obj* x_2, obj* x_3) {
+obj* l_DHashmap_empty___boxed(obj* x_0, obj* x_1, obj* x_2, obj* x_3) {
 _start:
 {
 obj* x_4; 
-x_4 = l_DHashmap_Empty(x_0, x_1, x_2, x_3);
+x_4 = l_DHashmap_empty(x_0, x_1, x_2, x_3);
 lean::dec(x_0);
 lean::dec(x_1);
 lean::dec(x_2);
@@ -1524,7 +1524,7 @@ lean::dec(x_3);
 return x_4;
 }
 }
-uint8 l_Hashmap_Empty___rarg(obj* x_0) {
+uint8 l_Hashmap_empty___rarg(obj* x_0) {
 _start:
 {
 obj* x_1; obj* x_2; uint8 x_3; 
@@ -1546,29 +1546,29 @@ return x_6;
 }
 }
 }
-obj* l_Hashmap_Empty(obj* x_0, obj* x_1, obj* x_2, obj* x_3) {
+obj* l_Hashmap_empty(obj* x_0, obj* x_1, obj* x_2, obj* x_3) {
 _start:
 {
 obj* x_4; 
-x_4 = lean::alloc_closure(reinterpret_cast<void*>(l_Hashmap_Empty___rarg___boxed), 1, 0);
+x_4 = lean::alloc_closure(reinterpret_cast<void*>(l_Hashmap_empty___rarg___boxed), 1, 0);
 return x_4;
 }
 }
-obj* l_Hashmap_Empty___rarg___boxed(obj* x_0) {
+obj* l_Hashmap_empty___rarg___boxed(obj* x_0) {
 _start:
 {
 uint8 x_1; obj* x_2; 
-x_1 = l_Hashmap_Empty___rarg(x_0);
+x_1 = l_Hashmap_empty___rarg(x_0);
 x_2 = lean::box(x_1);
 lean::dec(x_0);
 return x_2;
 }
 }
-obj* l_Hashmap_Empty___boxed(obj* x_0, obj* x_1, obj* x_2, obj* x_3) {
+obj* l_Hashmap_empty___boxed(obj* x_0, obj* x_1, obj* x_2, obj* x_3) {
 _start:
 {
 obj* x_4; 
-x_4 = l_Hashmap_Empty(x_0, x_1, x_2, x_3);
+x_4 = l_Hashmap_empty(x_0, x_1, x_2, x_3);
 lean::dec(x_0);
 lean::dec(x_1);
 lean::dec(x_2);
