src/stage0/init/data/rbtree/basic.cpp
@@ -79,6 +79,7 @@ obj* l_RBNode_findCore___main___at_RBTree_seteq___spec__4___boxed(obj*, obj*);
 obj* l_RBNode_mfold___main___at_RBTree_mfold___spec__1___rarg(obj*, obj*, obj*, obj*);
 obj* l_RBMap_findCore___main___at_RBTree_seteq___spec__3___rarg(obj*, obj*, obj*);
 obj* l_RBTree_contains___boxed(obj*, obj*);
+obj* l_RBTree_empty(obj*, obj*);
 obj* l_RBTree_toList___rarg(obj*);
 obj* l_RBNode_ins___main___at_rbtreeOf___spec__5___boxed(obj*, obj*);
 obj* l_RBTree_HasRepr___boxed(obj*, obj*);
@@ -99,6 +100,7 @@ obj* l_RBTree_find___at_RBTree_contains___spec__1___rarg(obj*, obj*, obj*);
 uint8 l_RBTree_any___rarg(obj*, obj*);
 obj* l_RBNode_balance2___main___rarg(obj*, obj*);
 obj* l_RBMap_insert___main___at_RBTree_ofList___main___spec__1___boxed(obj*, obj*);
+obj* l_RBTree_empty___boxed(obj*, obj*);
 obj* l_RBTree_fromList___rarg___boxed(obj*, obj*, obj*);
 obj* l_RBMap_findCore___main___at_RBTree_contains___spec__2___rarg(obj*, obj*, obj*);
 obj* l_RBMap_insert___main___at_RBTree_fromList___spec__2___rarg(obj*, obj*, obj*, obj*);
@@ -136,12 +138,11 @@ obj* l_RBMap_findCore___main___at_RBTree_contains___spec__2___boxed(obj*, obj*);
 obj* l_RBTree_fromList___boxed(obj*);
 obj* l_RBTree_subset___at_RBTree_seteq___spec__1___boxed(obj*, obj*);
 obj* l_RBTree_seteq(obj*, obj*);
-obj* l_RBTree_Empty(obj*, obj*);
 obj* l_RBTree_insert___at_RBTree_fromList___spec__1___boxed(obj*, obj*);
 obj* l_RBNode_all___main___at_RBTree_seteq___spec__10___rarg___boxed(obj*, obj*, obj*);
 obj* l_RBTree_revFold___boxed(obj*, obj*, obj*);
 obj* l_RBTree_find___at_RBTree_seteq___spec__7___boxed(obj*, obj*);
-obj* l_RBTree_Empty___rarg___boxed(obj*);
+obj* l_RBTree_empty___rarg___boxed(obj*);
 obj* l_RBNode_all___main___at_RBTree_seteq___spec__10___boxed(obj*, obj*);
 uint8 l_Option_toBool___main___rarg(obj*);
 obj* l_List_foldl___main___at_rbtreeOf___spec__7(obj*, obj*);
@@ -191,6 +192,7 @@ obj* l_RBTree_insert___at_rbtreeOf___spec__2___rarg(obj*, obj*, obj*);
 obj* l_RBMap_insert___main___at_RBTree_fromList___spec__2(obj*, obj*);
 obj* l_RBTree_fold(obj*, obj*, obj*);
 obj* l_RBNode_mfold___main___at_RBTree_mfor___spec__1___rarg(obj*, obj*, obj*, obj*);
+uint8 l_RBTree_empty___rarg(obj*);
 obj* l_RBNode_ins___main___at_RBTree_insert___spec__3___rarg(obj*, obj*, obj*, obj*);
 obj* l_RBNode_all___main___at_RBTree_all___spec__1___rarg___boxed(obj*, obj*);
 obj* l_RBTree_contains(obj*, obj*);
@@ -223,7 +225,6 @@ obj* l_RBNode_balance1___main___rarg(obj*, obj*);
 obj* l_RBTree_ofList___main___boxed(obj*, obj*);
 obj* l_RBNode_insert___at_RBTree_fromList___spec__3(obj*, obj*);
 obj* l_RBTree_depth(obj*, obj*);
-obj* l_RBTree_Empty___boxed(obj*, obj*);
 obj* l_RBMap_findCore___main___at_RBTree_subset___spec__2___rarg(obj*, obj*, obj*);
 obj* l_RBTree_fold___boxed(obj*, obj*, obj*);
 obj* l_RBTree_toList___boxed(obj*, obj*);
@@ -246,7 +247,6 @@ obj* l_RBNode_insert___at_RBTree_ofList___main___spec__2(obj*, obj*);
 obj* l_RBTree_subset___at_RBTree_seteq___spec__6___rarg___boxed(obj*, obj*, obj*);
 obj* l_List_repr___main___rarg(obj*, obj*);
 obj* l_RBNode_all___main___at_RBTree_subset___spec__4(obj*, obj*);
-uint8 l_RBTree_Empty___rarg(obj*);
 obj* l_RBTree_max(obj*, obj*);
 obj* l_RBNode_all___main___at_RBTree_all___spec__1___boxed(obj*);
 obj* l_RBNode_all___main___at_RBTree_seteq___spec__5___boxed(obj*, obj*);
@@ -680,7 +680,7 @@ lean::dec(x_3);
 return x_4;
 }
 }
-uint8 l_RBTree_Empty___rarg(obj* x_0) {
+uint8 l_RBTree_empty___rarg(obj* x_0) {
 _start:
 {
 if (lean::obj_tag(x_0) == 0)
@@ -697,29 +697,29 @@ return x_2;
 }
 }
 }
-obj* l_RBTree_Empty(obj* x_0, obj* x_1) {
+obj* l_RBTree_empty(obj* x_0, obj* x_1) {
 _start:
 {
 obj* x_2; 
-x_2 = lean::alloc_closure(reinterpret_cast<void*>(l_RBTree_Empty___rarg___boxed), 1, 0);
+x_2 = lean::alloc_closure(reinterpret_cast<void*>(l_RBTree_empty___rarg___boxed), 1, 0);
 return x_2;
 }
 }
-obj* l_RBTree_Empty___rarg___boxed(obj* x_0) {
+obj* l_RBTree_empty___rarg___boxed(obj* x_0) {
 _start:
 {
 uint8 x_1; obj* x_2; 
-x_1 = l_RBTree_Empty___rarg(x_0);
+x_1 = l_RBTree_empty___rarg(x_0);
 x_2 = lean::box(x_1);
 lean::dec(x_0);
 return x_2;
 }
 }
-obj* l_RBTree_Empty___boxed(obj* x_0, obj* x_1) {
+obj* l_RBTree_empty___boxed(obj* x_0, obj* x_1) {
 _start:
 {
 obj* x_2; 
-x_2 = l_RBTree_Empty(x_0, x_1);
+x_2 = l_RBTree_empty(x_0, x_1);
 lean::dec(x_0);
 lean::dec(x_1);
 return x_2;
