src/stage0/init/lean/parser/stringliteral.cpp
@@ -73,7 +73,6 @@ obj* l_Lean_Parser_MonadParsec_unexpectedAt___rarg(obj*, obj*, obj*, obj*);
 obj* l_Lean_Parser_parseQuotedChar___rarg___lambda__7___boxed(obj*, obj*, obj*, obj*, obj*, obj*);
 obj* l_Lean_Parser_parseQuotedChar___boxed(obj*, obj*);
 obj* l_Lean_Parser_parseHexDigit___rarg___lambda__4(obj*, obj*, obj*);
-obj* l_Dlist_singleton___rarg(obj*, obj*);
 obj* l_Lean_Parser_parseHexDigit(obj*, obj*);
 obj* l_Lean_Parser_parseHexDigit___rarg___closed__1;
 obj* l_Lean_Parser_parseQuotedChar___rarg___lambda__4(obj*, obj*, obj*, obj*);
@@ -85,6 +84,7 @@ obj* l_Lean_Parser_parseStringLiteral___rarg___lambda__2___boxed(obj*, obj*, obj
 extern obj* l_Lean_Parser_MonadParsec_leftOver___rarg___closed__1;
 obj* l_Lean_Parser_parseStringLiteral___rarg___lambda__1(obj*, obj*, obj*, obj*);
 obj* l_Lean_Parser_parseQuotedChar___rarg___lambda__3(obj*, obj*, obj*, obj*, obj*);
+obj* l_DList_singleton___rarg(obj*, obj*);
 obj* l_Lean_Parser_parseStringLiteralAux___main___rarg(obj*, obj*, obj*, obj*, obj*);
 obj* l_Lean_Parser_MonadParsec_labels___rarg___lambda__1___boxed(obj*, obj*, obj*, obj*, obj*, obj*);
 namespace lean {
@@ -331,7 +331,7 @@ _start:
 {
 obj* x_0; obj* x_1; obj* x_2; 
 x_0 = lean::mk_string("hexadecimal");
-x_1 = lean::alloc_closure(reinterpret_cast<void*>(l_Dlist_singleton___rarg), 2, 1);
+x_1 = lean::alloc_closure(reinterpret_cast<void*>(l_DList_singleton___rarg), 2, 1);
 lean::closure_set(x_1, 0, x_0);
 x_2 = lean::alloc_closure(reinterpret_cast<void*>(l_Lean_Parser_MonadParsec_labels___rarg___lambda__1___boxed), 6, 1);
 lean::closure_set(x_2, 0, x_1);
