library/init/data/array/basic.lean
@@ -35,13 +35,13 @@ rfl
 namespace Array
 variables {α : Type u} {β : Type v}
 
-@[extern cpp inline "lean::mk_nil_array()"]
-def mkNil (_ : Unit) : Array α :=
+@[extern cpp inline "lean::mk_empty_array()"]
+def mkEmpty (_ : Unit) : Array α :=
 { sz   := 0,
   data := λ ⟨x, h⟩, absurd h (Nat.notLtZero x) }
 
 def empty : Array α :=
-mkNil ()
+mkEmpty ()
 
 instance : HasEmptyc (Array α) :=
 ⟨Array.empty⟩
@@ -49,41 +49,41 @@ instance : HasEmptyc (Array α) :=
 def isEmpty (a : Array α) : Bool :=
 a.size = 0
 
-@[extern cpp inline "lean::array_read(#2, #3)"]
-def read (a : @& Array α) (i : @& Fin a.sz) : α :=
+@[extern cpp inline "lean::array_index(#2, #3)"]
+def index (a : @& Array α) (i : @& Fin a.sz) : α :=
 a.data i
 
-@[extern cpp inline "lean::array_write(#2, #3, #4)"]
-def write (a : Array α) (i : @& Fin a.sz) (v : α) : Array α :=
+/- Low-level version of `index` which is as fast as a C array read.
+   `Fin` values are represented as tag pointers in the Lean runtime. Thus,
+   `index` may be slightly slower than `idx`. -/
+@[extern cpp inline "lean::array_idx(#2, #3)"]
+def idx (a : @& Array α) (i : USize) (h : i.toNat < a.sz) : α :=
+a.index ⟨i.toNat, h⟩
+
+/- "Comfortable" version of `index`. It performs a bound check at runtime. -/
+@[extern cpp inline "lean::array_get(#2, #3, #4)"]
+def get [Inhabited α] (a : @& Array α) (i : @& Nat) : α :=
+if h : i < a.sz then a.index ⟨i, h⟩ else default α
+
+@[extern cpp inline "lean::array_update(#2, #3, #4)"]
+def update (a : Array α) (i : @& Fin a.sz) (v : α) : Array α :=
 { sz   := a.sz,
   data := λ j, if h : i = j then v else a.data j }
 
-theorem szWriteEq (a : Array α) (i : Fin a.sz) (v : α) : (write a i v).sz = a.sz :=
+/- Low-level version of `update` which is as fast as a C array update.
+   `Fin` values are represented as tag pointers in the Lean runtime. Thus,
+   `update` may be slightly slower than `updt`. -/
+@[extern cpp inline "lean::array_updt(#2, #3, #4)"]
+def updt (a : @& Array α) (i : USize) (v : @& α) (h : i.toNat < a.sz) : Array α :=
+a.update ⟨i.toNat, h⟩ v
+
+/- "Comfortable" version of `update`. It performs a bound check at runtime. -/
+@[extern cpp inline "lean::array_set(#2, #3, #4)"]
+def set (a : Array α) (i : @& Nat) (v : α) : Array α :=
+if h : i < a.sz then a.update ⟨i, h⟩ v else a
+
+theorem szUpdateEq (a : Array α) (i : Fin a.sz) (v : α) : (update a i v).sz = a.sz :=
 rfl
-
-@[extern cpp inline "lean::array_safe_read(#2, #3, #4)"]
-def read' [Inhabited α] (a : @& Array α) (i : @& Nat) : α :=
-if h : i < a.sz then a.read ⟨i, h⟩ else default α
-
-@[extern cpp inline "lean::array_safe_write(#2, #3, #4)"]
-def write' (a : Array α) (i : @& Nat) (v : α) : Array α :=
-if h : i < a.sz then a.write ⟨i, h⟩ v else a
-
-@[extern cpp inline "lean::array_uread(#2, #3)"]
-def uread (a : @& Array α) (i : USize) (h : i.toNat < a.sz) : α :=
-a.read ⟨i.toNat, h⟩
-
-@[extern cpp inline "lean::array_uwrite(#2, #3, #4)"]
-def uwrite (a : @& Array α) (i : USize) (v : @& α) (h : i.toNat < a.sz) : Array α :=
-a.write ⟨i.toNat, h⟩ v
-
-@[extern cpp inline "lean::array_safe_uread(#2, #3, #4)"]
-def uread' [Inhabited α] (a : Array α) (i : USize) : α :=
-if h : i.toNat < a.sz then a.read ⟨i.toNat, h⟩ else default α
-
-@[extern cpp inline "lean::array_safe_uwrite(#2, #3, #4)"]
-def uwrite' (a : Array α) (i : USize) (v : α) : Array α :=
-if h : i.toNat < a.sz then a.write ⟨i.toNat, h⟩ v else a
 
 @[extern cpp inline "lean::array_push(#2, #3)"]
 def push (a : Array α) (v : α) : Array α :=
@@ -95,14 +95,14 @@ def push (a : Array α) (v : α) : Array α :=
 @[extern cpp inline "lean::array_pop(#2)"]
 def pop (a : Array α) : Array α :=
 { sz   := Nat.pred a.sz,
-  data := λ ⟨j, h⟩, a.read ⟨j, Nat.ltOfLtOfLe h (Nat.predLe _)⟩ }
+  data := λ ⟨j, h⟩, a.index ⟨j, Nat.ltOfLtOfLe h (Nat.predLe _)⟩ }
 
 -- TODO(Leo): justify termination using wf-rec
 @[specialize] private def iterateAux (a : Array α) (f : Π i : Fin a.sz, α → β → β) : Nat → β → β
 | i b :=
   if h : i < a.sz then
      let idx : Fin a.sz := ⟨i, h⟩ in
-     iterateAux (i+1) (f idx (a.read idx) b)
+     iterateAux (i+1) (f idx (a.index idx) b)
   else b
 
 @[inline] def iterate (a : Array α) (b : β) (f : Π i : Fin a.sz, α → β → β) : β :=
@@ -115,7 +115,7 @@ iterate a b (λ _, f)
 | 0     h b := b
 | (j+1) h b :=
   let i : Fin a.sz := ⟨j, h⟩ in
-  revIterateAux j (Nat.leOfLt h) (f i (a.read i) b)
+  revIterateAux j (Nat.leOfLt h) (f i (a.index i) b)
 
 @[inline] def revIterate (a : Array α) (b : β) (f : Π i : Fin a.sz, α → β → β) : β :=
 revIterateAux a f a.size (Nat.leRefl _) b
@@ -135,7 +135,7 @@ instance [HasToString α] : HasToString (Array α) :=
 @[inline] private def foreachAux (a : Array α) (f : Π i : Fin a.sz, α → α) : { a' : Array α // a'.sz = a.sz } :=
 iterate a ⟨a, rfl⟩ $ λ i v ⟨a', h⟩,
   let i' : Fin a'.sz := Eq.recOn h.symm i in
-  ⟨a'.write i' (f i v), (szWriteEq a' i' (f i v)) ▸ h⟩
+  ⟨a'.update i' (f i v), (szUpdateEq a' i' (f i v)) ▸ h⟩
 
 @[inline] def foreach (a : Array α) (f : Π i : Fin a.sz, α → α) : Array α :=
 (foreachAux a f).val
@@ -148,8 +148,8 @@ foreach a (λ _, f)
 
 @[inline] def map₂ (f : α → α → α) (a b : Array α) : Array α :=
 if h : a.size ≤ b.size
-then foreach a (λ ⟨i, h'⟩, f (b.read ⟨i, Nat.ltOfLtOfLe h' h⟩))
-else foreach b (λ ⟨i, h'⟩, f (a.read ⟨i, Nat.ltTrans h' (Nat.gtOfNotLe h)⟩))
+then foreach a (λ ⟨i, h'⟩, f (b.index ⟨i, Nat.ltOfLtOfLe h' h⟩))
+else foreach b (λ ⟨i, h'⟩, f (a.index ⟨i, Nat.ltTrans h' (Nat.gtOfNotLe h)⟩))
 
 end Array
 
